\documentclass{report}
\usepackage{amssymb,latexsym,amsmath,array}
\usepackage{graphicx}
\setlength{\oddsidemargin}{-.5in}
\setlength{\evensidemargin}{-.5in} 
\setlength{\textwidth}{7in}
\newtheorem{theorem}{Theorem}
\newtheorem{definition}{Definition}
\newtheorem{notation}{Notation}
\addtolength{\topmargin}{-1.5in}
\addtolength{\textheight}{1.5in}

\begin{document}
\begin{center}
\textbf{M. Steven Towns}\\
Assignment \# 2\\
\today\\
Linear Algebra\\

\end{center}
\hrulefill

$\newline$

\section*{Problem 25:}
If $A = \bigl[ a_{ij} \bigr]$ is an $n \times m$ matrix, then the \textbf{trace} of $A$, $Tr(A)$, is defined as the sum of all the elements on the main diagonal of $A$, $Tr(A) = \sum_{i=1}^{n} a_{ii}$. Prove: 
\newline
\newline

(a) $Tr(cA)=cTr(A)$, where $c$ is a real number. 
	\begin{center}
		$
			\sum\limits_{i=1}^n (ca_{ii}) = ca_{11} + ca_{22} + \cdots + ca_{nn}
		$
	\end{center}
	\begin{center}
		$
			= c(a_{11} + a_{22} + \cdots + a_{nn}) = c\sum\limits_{i=1}^n (a_{ii})
		$
	\end{center}

(b) $Tr(A + B)=Tr(A) + Tr(B)$
	\begin{center}
		$
			\sum\limits_{i=1}^n (a_{ii} + b_{ii}) = a_{11} + b_{11} + a_{22} + b_{22} + \cdots + a_{nn} + b_{nn}
		$
	\end{center}
	\begin{center}
		$
			= (a_{11} + a_{22} + \cdots + a_{nn})+ (b_{11} + b_{22} + \cdots + b_{nn})
		$
	\end{center}
	\begin{center}
		$
			= \sum\limits_{i=1}^n(a_{ii})+\sum\limits_{i=1}^n(b_{ii})
		$
	\end{center}

(c) $Tr(AB)=Tr(BA)$
	\begin{center}
		$
			\sum\limits_{i=1}^n\sum\limits_{i=1}^m(a_{im}b_{mi}) = \sum\limits_{i=1}^n(a_{11}b_{11} + a_{22}b_{22} + \cdots + a_{mm}b_{nn})
		$
	\end{center}

	\begin{center}
		$
			= \sum\limits_{i=1}^n(b_{11}a_{11} + b_{22}a_{22} + \cdots + b_{nn}a_{mm}) = \sum\limits_{i=1}^n\sum\limits_{i=1}^m(b_{mi}a_{im})
		$
	\end{center}

(d) $Tr(A^T)=Tr(A)$

	\begin{center}
		$
			\sum\limits_{i=1}^{n}(a_{ii}) = a_{11} + a_{22} + \cdots + a_{nn}
		$ 
	\end{center}
	\begin{center}
		$
			= (a_{11})^T + (a_{22})^T + \cdots + (a_{nn})^T = \sum\limits_{i=1}^n(a_{ii})^T
		$ 
	\end{center}


(e) $Tr(A^TA) \geq 0$
	\begin{center}
		 $
		 	Tr(A^T)=Tr(A) \therefore Tr(A^TA)=Tr(A^2)
		 $
	\end{center}
	
	\begin{center}
		$Tr(A^2) = \sum\limits_{i=1}^n(a_{ii})^2$
	\end{center}
	
	\begin{center}
		$
			\sum\limits_{i=1}^n(a_{ii})^2=(a_{11})^2 + (a_{22})^2 + \cdots + (a_{nn})^2
		$
	\end{center}
	\begin{center}
		$
			a_{ii} \in \mathbb{R} \therefore (a_{ii})^2 \geq 0
		$
	\end{center}
	\begin{center}
		$
			\therefore \sum\limits_{i=1}^n(a_{ii})^2 \geq 0
		$
	\end{center}
	
	


\end{document}