\documentclass{report}
\usepackage{amssymb,latexsym,amsmath,array}
\usepackage{graphicx}
\setlength{\oddsidemargin}{-.5in}
\setlength{\evensidemargin}{-.5in} 
\setlength{\textwidth}{7in}
\newtheorem{theorem}{Theorem}
\newtheorem{definition}{Definition}
\newtheorem{notation}{Notation}
\addtolength{\topmargin}{-1.5in}
\addtolength{\textheight}{1.5in}

\begin{document}
\begin{center}
\textbf{M. Steven Towns}\\
Assignment \# 2\\
\today\\
Linear Algebra\\

\end{center}
\hrulefill
\section*{Proof:}
Prove that
$
	\sum\limits_{j=1}^n \sum\limits_{i=1}^m(a_{ij})=
	\sum\limits_{i=1}^m \sum\limits_{j=1}^n(a_{ij})
$
\\
\begin{center}
	Left:
	\\
	$
		\sum\limits_{j=1}^n \sum\limits_{i=1}^m(a_{ij})=
		$
		\\
		$
		\sum\limits_{j=1}^n(a_{1j}+a_{2j}+\hdots+a_{mj})=
	$
\\
	$
		\begin{bmatrix}
			a_{11} & a_{21} & \hdots & a_{m1}\\
			a_{12} & a_{22} & \hdots & a_{m2}\\
			\vdots & \vdots &  & \vdots\\
			a_{1n} & a_{2n} & \hdots & a_{mn}
		\end{bmatrix}
	$
\end{center}
\begin{center}
\end{center}
\begin{center}
	Right:\\
	$
		\sum\limits_{i=1}^m \sum\limits_{j=1}^n(a_{ij})=
	$
	\\
	$
		\sum\limits_{i=1}^n(a_{i1}+a_{i2}+\hdots+a_{in})=
	$
	\\
	$
		\begin{bmatrix}
			a_{11} & a_{21} & \hdots & a_{m1}\\
			a_{12} & a_{22} & \hdots & a_{m2}\\
			\vdots & \vdots &  & \vdots\\
			a_{1n} & a_{2n} & \hdots & a_{mn}
		\end{bmatrix}
	$\\
	The two matrices are equal $\therefore $ 
	$
		\sum\limits_{j=1}^n \sum\limits_{i=1}^m(a_{ij})=
		\sum\limits_{i=1}^m \sum\limits_{j=1}^n(a_{ij})
	$
\end{center}
\end{document}